backend/Renumberproof.v
@@ -18,38 +18,87 @@ Require Import Postorder.
 Require Import Events.
 Require Import Globalenvs.
 Require Import Smallstep.
+Require Import Language.
 Require Import Op.
 Require Import Registers.
 Require Import RTL.
 Require Import Renumber.
+Require Import Linkeq.
+Require Import SepcompRel.
+Require Import RTLExtra.
+Require Import sflib.
+
+Inductive match_fundef: forall (fd fd': fundef), Prop :=
+| match_fundef_transl fd fd'
+    (FD: transf_fundef fd = fd'):
+    match_fundef fd fd'
+| match_fundef_identical fd:
+    match_fundef fd fd.
 
 Section PRESERVATION.
 
 Variable prog: program.
-Let tprog := transf_program prog.
+Variable tprog: program.
+Hypothesis TRANSF:
+  @sepcomp_rel
+    Language_RTL Language_RTL
+    (fun p f tf => transf_function f = tf \/ f = tf)
+    (fun p ef tef => ef = tef)
+    (@Errors.OK _)
+    prog tprog.
 Let ge := Genv.globalenv prog.
 Let tge := Genv.globalenv tprog.
 
 Lemma functions_translated:
   forall v f,
   Genv.find_funct ge v = Some f ->
-  Genv.find_funct tge v = Some (transf_fundef f).
-Proof (@Genv.find_funct_transf _ _ _ transf_fundef prog).
+  exists tf, Genv.find_funct tge v = Some tf /\ (match_fundef f tf).
+Proof.
+  generalize (find_funct_transf_optionally _ _ TRANSF).
+  intros H1 v f. specialize (H1 v f).
+  revert H1. unfold ge, fundef. simpl.
+  match goal with
+    | [|- _ -> ?a = _ -> _] => destruct a
+  end; intros H1 H2; inv H2.
+  specialize (H1 eq_refl). destruct H1 as [? [? H1]].
+  exists x.
+  split; auto.
+  destruct H1 as [[prog1 [_ H1]] | H1].
+  + destruct f.
+    * constructor; auto.
+    * rewrite H1; apply match_fundef_identical.
+  + rewrite H1; apply match_fundef_identical.
+Qed.
 
 Lemma function_ptr_translated:
   forall v f,
   Genv.find_funct_ptr ge v = Some f ->
-  Genv.find_funct_ptr tge v = Some (transf_fundef f).
-Proof (@Genv.find_funct_ptr_transf _ _ _ transf_fundef prog).
+  exists tf, Genv.find_funct_ptr tge v = Some tf /\ (match_fundef f tf).
+Proof.
+  generalize (find_funct_ptr_transf_optionally _ _ TRANSF).
+  intros H1 v f. specialize (H1 v f).
+  revert H1. unfold ge, fundef. simpl.
+  match goal with
+    | [|- _ -> ?a = _ -> _] => destruct a
+  end; intros H1 H2; inv H2.
+  specialize (H1 eq_refl). destruct H1 as [? [? H1]].
+  exists x.
+  split; auto.
+  destruct H1 as [[prog1 [_ H1]] | H1].
+  + destruct f.
+    * constructor; auto.
+    * rewrite H1; apply match_fundef_identical.
+  + rewrite H1; apply match_fundef_identical.
+Qed.
 
 Lemma symbols_preserved:
   forall id,
   Genv.find_symbol tge id = Genv.find_symbol ge id.
-Proof (@Genv.find_symbol_transf _ _ _ transf_fundef prog).
+Proof (find_symbol_transf_optionally _ _ TRANSF).
 
 Lemma varinfo_preserved:
   forall b, Genv.find_var_info tge b = Genv.find_var_info ge b.
-Proof (@Genv.find_var_info_transf _ _ _ transf_fundef prog).
+Proof (find_var_info_transf_optionally _ _ TRANSF).
 
 Lemma sig_preserved:
   forall f, funsig (transf_fundef f) = funsig f.
@@ -57,10 +106,19 @@ Proof.
   destruct f; reflexivity.
 Qed.
 
+Lemma match_fundef_sig:
+  forall f1 f2 (MATCHFD: match_fundef f1 f2), funsig f2 = funsig f1.
+Proof.
+  intros. inv MATCHFD; auto.
+  eapply sig_preserved.
+Qed.
+
 Lemma find_function_translated:
   forall ros rs fd,
   find_function ge ros rs = Some fd ->
-  find_function tge ros rs = Some (transf_fundef fd).
+  exists tfd,
+    <<TFD: find_function tge ros rs = Some tfd>> /\
+    <<MATCH: match_fundef fd tfd>>.
 Proof.
   unfold find_function; intros. destruct ros as [r|id]. 
   eapply functions_translated; eauto.
@@ -135,7 +193,16 @@ Inductive match_frames: RTL.stackframe -> RTL.stackframe -> Prop :=
   | match_frames_intro: forall res f sp pc rs
         (REACH: reach f pc),
       match_frames (Stackframe res f sp pc rs)
-                   (Stackframe res (transf_function f) sp (renum_pc (pnum f) pc) rs).
+                   (Stackframe res (transf_function f) sp (renum_pc (pnum f) pc) rs)
+  | match_frames_identical : forall res f sp pc rs,
+      match_frames (Stackframe res f sp pc rs)
+                   (Stackframe res f sp pc rs).
+
+Inductive match_identical_states: RTL.state -> RTL.state -> Prop :=
+  | match_identical_regular_states: forall stk f sp pc rs m stk'
+        (STACKS: list_forall2 match_frames stk stk'),
+      match_identical_states (State stk f sp pc rs m)
+                   (State stk' f sp pc rs m).
 
 Inductive match_states: RTL.state -> RTL.state -> Prop :=
   | match_regular_states: forall stk f sp pc rs m stk'
@@ -143,21 +210,57 @@ Inductive match_states: RTL.state -> RTL.state -> Prop :=
         (REACH: reach f pc),
       match_states (State stk f sp pc rs m)
                    (State stk' (transf_function f) sp (renum_pc (pnum f) pc) rs m)
-  | match_callstates: forall stk f args m stk'
+  | match_callstates: forall stk f args m stk' f'
+        (FD: match_fundef f f')
         (STACKS: list_forall2 match_frames stk stk'),
       match_states (Callstate stk f args m)
-                   (Callstate stk' (transf_fundef f) args m)
+                   (Callstate stk' f' args m)
   | match_returnstates: forall stk v m stk'
         (STACKS: list_forall2 match_frames stk stk'),
       match_states (Returnstate stk v m)
-                   (Returnstate stk' v m).
+                   (Returnstate stk' v m)
+  | match_states_identical: forall s s'
+        (MATCH: match_identical_states s s'),
+      match_states s s'.
+
+Lemma step_simulation_identical:
+  forall S1 t S2, RTL.step ge S1 t S2 ->
+  forall S1' (MS: match_identical_states S1 S1'),
+  exists S2', RTL.step tge S1' t S2' /\ match_states S2 S2'.
+Proof.
+  intros. destruct (is_normal S1) eqn:NORMAL1.
+  { (* is_normal *)
+    destruct S1; try by inv NORMAL1.
+    exploit is_normal_step; eauto. i;des. subst.
+    inv MS. exploit is_normal_identical; eauto using symbols_preserved, varinfo_preserved.
+    i; des. esplits; eauto.
+    apply match_states_identical. econs; eauto.
+  }
+  inv MS. unfold is_normal in NORMAL1.
+  destruct (fn_code f) ! pc as [[]|] eqn:OPCODE; try by inv NORMAL1; inv H; clarify.
+  - (* Icall *)
+    inv H; clarify.
+    exploit find_function_translated; eauto. i; des.
+    esplits; eauto using exec_Icall, match_fundef_sig.
+    econs; eauto. constructor; eauto using match_frames_identical.
+  - (* Itailcall *)
+    inv H; clarify.
+    exploit find_function_translated; eauto. i; des.
+    esplits; eauto using exec_Itailcall, match_fundef_sig. econs; eauto.
+  - (* Ireturn *)
+    inv H; clarify.
+    esplits; eauto using exec_Ireturn. econs; eauto.
+Qed.
 
 Lemma step_simulation:
   forall S1 t S2, RTL.step ge S1 t S2 ->
   forall S1', match_states S1 S1' ->
   exists S2', RTL.step tge S1' t S2' /\ match_states S2 S2'.
 Proof.
-  induction 1; intros S1' MS; inv MS; try TR_AT.
+  intros s1 t s2 BACKUP_STEP. generalize BACKUP_STEP.
+  induction 1; intros S1' MS; inv MS;
+  try (by eauto using step_simulation_identical); try TR_AT.
+
 (* nop *)
   econstructor; split. eapply exec_Inop; eauto. 
   constructor; auto. eapply reach_succ; eauto. simpl; auto. 
@@ -179,17 +282,19 @@ Proof.
   eapply exec_Istore; eauto.
   constructor; auto. eapply reach_succ; eauto. simpl; auto.
 (* call *)
+  exploit find_function_translated; eauto. i. des.
   econstructor; split.
-  eapply exec_Icall with (fd := transf_fundef fd); eauto.
-    eapply find_function_translated; eauto.
+  eapply exec_Icall with (fd := tfd); eauto.
+    inv MATCH; auto.
     apply sig_preserved.
-  constructor. constructor; auto. constructor. eapply reach_succ; eauto. simpl; auto.
+  constructor; auto. constructor; auto. constructor; auto. eapply reach_succ; eauto. simpl; auto.
 (* tailcall *)
+  exploit find_function_translated; eauto. i. des.
   econstructor; split.
-  eapply exec_Itailcall with (fd := transf_fundef fd); eauto.
-    eapply find_function_translated; eauto.
+  eapply exec_Itailcall with (fd := tfd); eauto.
+    inv MATCH; auto.
     apply sig_preserved.
-  constructor. auto.
+  constructor; auto.
 (* builtin *)
   econstructor; split.
   eapply exec_Ibuiltin; eauto.
@@ -212,10 +317,17 @@ Proof.
   eapply exec_Ireturn; eauto. 
   constructor; auto.
 (* internal function *)
+  inv FD.
+  (* call translated *)
   simpl. econstructor; split.
   eapply exec_function_internal; eauto. 
   constructor; auto. unfold reach. constructor. 
+  (* call identical *)
+  simpl. econstructor; split.
+  eapply exec_function_internal; eauto.
+  apply match_states_identical. constructor; auto.
 (* external function *)
+  assert (f' = AST.External ef) by (inv FD; auto). subst.
   econstructor; split.
   eapply exec_function_external; eauto.
     eapply external_call_symbols_preserved; eauto.
@@ -223,8 +335,14 @@ Proof.
   constructor; auto.
 (* return *)
   inv STACKS. inv H1.
+  (* transl *)
   econstructor; split. 
   eapply exec_return; eauto. 
+  constructor; auto.
+  (* identical *)
+  econstructor; split. 
+  eapply exec_return; eauto.
+  apply match_states_identical.
   constructor; auto.
 Qed.
 
@@ -232,19 +350,23 @@ Lemma transf_initial_states:
   forall S1, RTL.initial_state prog S1 ->
   exists S2, RTL.initial_state tprog S2 /\ match_states S1 S2.
 Proof.
-  intros. inv H. econstructor; split.
+  intros. inv H.
+  exploit function_ptr_translated; eauto. i. des.
+  econstructor; split.
   econstructor. 
-    eapply Genv.init_mem_transf; eauto. 
-    simpl. rewrite symbols_preserved. eauto. 
-    eapply function_ptr_translated; eauto. 
+    eapply (init_mem_transf_optionally _ _ TRANSF); eauto. 
+    replace (AST.prog_main tprog) with (AST.prog_main prog); [|by inv TRANSF; auto].
+    rewrite symbols_preserved. eauto. 
+    eauto. inv H4; auto.
     rewrite <- H3; apply sig_preserved.
-  constructor. constructor.
+  constructor; auto. constructor.
 Qed.
 
 Lemma transf_final_states:
   forall S1 S2 r, match_states S1 S2 -> RTL.final_state S1 r -> RTL.final_state S2 r.
 Proof.
   intros. inv H0. inv H. inv STACKS. constructor.
+  inv MATCH.
 Qed.
 
 Theorem transf_program_correct:
@@ -259,9 +381,20 @@ Qed.
 
 End PRESERVATION.
 
-
-
- 
-
-  
-
+Lemma Renumber_sepcomp_rel
+      rtlprog1 rtlprog2
+      (Htrans: Renumber.transf_program rtlprog1 = rtlprog2 \/ rtlprog1 = rtlprog2):
+  @sepcomp_rel
+    Language.Language_RTL Language.Language_RTL
+    (fun p f tf => Renumber.transf_function f = tf \/ f = tf)
+    (fun p ef tef => ef = tef)
+    (@Errors.OK _)
+    rtlprog1 rtlprog2.
+Proof.
+  inv Htrans.
+  - apply transf_program_optionally_sepcomp_rel.
+    unfold Renumber.transf_program. f_equal.
+    apply Axioms.functional_extensionality. intro fd.
+    destruct fd; auto.
+  - apply transf_program_optionally_sepcomp_rel_identical. auto.
+Qed.
