driver/CompilerExtra.v
@@ -1,0 +1,203 @@
+(* *********************************************************************)
+(*                                                                     *)
+(*              The Compcert verified compiler                         *)
+(*                                                                     *)
+(*          Xavier Leroy, INRIA Paris-Rocquencourt                     *)
+(*                                                                     *)
+(*  Copyright Institut National de Recherche en Informatique et en     *)
+(*  Automatique.  All rights reserved.  This file is distributed       *)
+(*  under the terms of the INRIA Non-Commercial License Agreement.     *)
+(*                                                                     *)
+(* *********************************************************************)
+
+(** The whole compiler and its proof of semantic preservation *)
+
+(** Libraries. *)
+Require Import String.
+Require Import Coqlib.
+Require Import Errors.
+Require Import AST.
+Require Import Smallstep.
+(** Languages (syntax and semantics). *)
+Require Csyntax.
+Require Csem.
+Require Cstrategy.
+Require Cexec.
+Require Clight.
+Require Csharpminor.
+Require Cminor.
+Require CminorSel.
+Require RTL.
+Require LTL.
+Require Linear.
+Require Mach.
+Require Asm.
+(** Translation passes. *)
+Require Initializers.
+Require SimplExpr.
+Require SimplLocals.
+Require Cshmgen.
+Require Cminorgen.
+Require Selection.
+Require RTLgen.
+Require Tailcall.
+Require Inlining.
+Require Renumber.
+Require Constprop.
+Require CSE.
+Require Deadcode.
+Require Allocation.
+Require Tunneling.
+Require Linearize.
+Require CleanupLabels.
+Require Stacking.
+Require Asmgen.
+(** Proofs of semantic preservation. *)
+Require SimplExprproof.
+Require SimplLocalsproof.
+Require Cshmgenproof.
+Require Cminorgenproof.
+Require Selectionproof.
+Require RTLgenproof.
+Require Tailcallproof.
+Require Inliningproof.
+Require Renumberproof.
+Require Constpropproof.
+Require CSEproof.
+Require Deadcodeproof.
+Require Allocproof.
+Require Tunnelingproof.
+Require Linearizeproof.
+Require CleanupLabelsproof.
+Require Stackingproof.
+Require Asmgenproof.
+Require Import Compiler.
+Require Import sflib.
+
+Definition transf_cminor_program_to_rtl (p: Cminor.program) : res RTL.program :=
+   OK p
+   @@ print print_Cminor
+  @@@ time "Instruction selection" Selection.sel_program
+  @@@ time "RTL generation" RTLgen.transl_program.
+
+Definition transf_clight_program_to_rtl (p: Clight.program) : res RTL.program :=
+  OK p 
+   @@ print print_Clight
+  @@@ time "Simplification of locals" SimplLocals.transf_program
+  @@@ time "C#minor generation" Cshmgen.transl_program
+  @@@ time "Cminor generation" Cminorgen.transl_program
+  @@@ transf_cminor_program_to_rtl.
+
+Definition transf_c_program_to_rtl (p: Csyntax.program) : res RTL.program :=
+  OK p 
+  @@@ time "Clight generation" SimplExpr.transl_program
+  @@@ transf_clight_program_to_rtl.
+
+Definition transf_rtl_program_to_asm (f: RTL.program) : res Asm.program :=
+   OK f
+   @@ print (print_RTL 0)
+   @@@ time "Register allocation" Allocation.transf_program
+   @@ print print_LTL
+   @@ time "Branch tunneling" Tunneling.tunnel_program
+  @@@ Linearize.transf_program
+   @@ time "Label cleanup" CleanupLabels.transf_program
+  @@@ time "Mach generation" Stacking.transf_program
+   @@ print print_Mach
+  @@@ time "Asm generation" Asmgen.transf_program.
+
+Inductive optimize_rtl_program: forall (rtl: RTL.program) (ortl: RTL.program), Prop:=
+| rtlopt_tailcall: forall r1,
+                     optimize_rtl_program r1 (Tailcall.transf_program r1)
+| rtlopt_inlining: forall r1 r1' (TR_OK: Inlining.transf_program r1 = OK r1'),
+                     optimize_rtl_program r1 r1'
+| rtlopt_renumber: forall r1,
+                     optimize_rtl_program r1 (Renumber.transf_program r1)
+| rtlopt_constprop: forall r1,
+                      optimize_rtl_program r1 (Constprop.transf_program r1)
+| rtlopt_cse: forall r1 r1' (TR_OK: CSE.transf_program r1 = OK r1'),
+                optimize_rtl_program r1 r1'
+| rtlopt_deadcode: forall r1 r1' (TR_OK: Deadcode.transf_program r1 = OK r1'),
+                     optimize_rtl_program r1 r1'.
+
+Definition compile_c_program (c: Csyntax.program) (a:Asm.program) : Prop :=
+  exists rtl ortl,
+    transf_c_program_to_rtl c = OK rtl
+    /\ (rtc optimize_rtl_program) rtl ortl
+    /\ transf_rtl_program_to_asm ortl = OK a.
+
+Ltac simplify:=
+  match goal with
+    | H: match ?x with
+           | OK _ => _
+           | Error _ => Error _
+         end = OK _
+      |- _ => (destruct x eqn:?D;[|inv H])
+    | H: OK _ = OK _ |- _ => inv H
+  end.
+
+Lemma transf_c_program_compile_c_program:
+  forall p tp
+         (Htrans: transf_c_program p = OK tp),
+    compile_c_program p tp.
+Proof.
+  intros.
+  unfold transf_c_program in Htrans.
+  unfold transf_clight_program in Htrans.
+  unfold transf_cminor_program in Htrans.
+  unfold Compiler.time, Compiler.print in Htrans.
+  unfold Compiler.apply_partial, Compiler.apply_total in Htrans.
+
+  unfold compile_c_program.
+  unfold transf_c_program_to_rtl.
+  unfold transf_clight_program_to_rtl.
+  unfold transf_cminor_program_to_rtl.
+  unfold time, print, apply_partial, apply_total.
+
+  destruct (SimplExpr.transl_program p); [|inversion Htrans].
+  destruct (SimplLocals.transf_program p0); [|inversion Htrans].
+  destruct (Cshmgen.transl_program p1); [|inversion Htrans].
+  destruct (Cminorgen.transl_program p2); [|inversion Htrans].
+  destruct (Selection.sel_program p3); [|inversion Htrans].
+  destruct (RTLgen.transl_program p4); [|inversion Htrans].
+  exists p5. clear -Htrans.
+
+  unfold transf_rtl_program in Htrans.
+  unfold Compiler.time, Compiler.apply_partial, Compiler.apply_total, Compiler.print in Htrans.
+  repeat simplify.
+
+  unfold Compiler.total_if, Compiler.partial_if in *.
+  eexists. split; auto.
+  split.
+  - assert (Hr1: rtc optimize_rtl_program p5 p17).
+    { destruct (Compopts.optim_tailcalls tt).
+      - econs 3; econs 1; [econs 1 | econs 2; eauto].
+      - econs 1. econs 2. eauto.
+    }
+    assert (Hr2: rtc optimize_rtl_program p17 p9).
+    { destruct (Compopts.optim_CSE tt).
+      - destruct (Compopts.optim_constprop tt).
+        + econs 3. econs 1. econs 3.
+          econs 3. econs 1. econs 4.
+          econs 3. econs 1. econs 3.
+          econs 1. econs 5. eauto.
+        + econs 3. econs 1. econs 3.
+          econs 1. econs 5. eauto.
+      - destruct (Compopts.optim_constprop tt).
+        + econs 3. econs 1. econs 3.
+          econs 3. econs 1. econs 4.
+          econs 1. inv D9. econs 3.
+        + econs 1. inv D9. econs 3.
+    }
+    assert (Hr3: rtc optimize_rtl_program p9 p7).
+    { destruct (Compopts.optim_redundancy tt).
+      - econs 1. econs 6. eauto.
+      - inv D7. econs 2.
+    }
+    econs 3; econs 3; eauto.
+  - clear -D0 D2 D5 Htrans.
+    unfold transf_rtl_program_to_asm.
+    unfold apply_partial, apply_total.
+    unfold time, print.
+    destruct (Allocation.transf_program p7); [|inv D5]. simplify.
+    rewrite D2, D0. auto.
+Qed.
