driver/Linkerproof.v
@@ -1,0 +1,328 @@
+Require Import Axioms.
+Require Import RelationClasses.
+Require String.
+Require Import Coqlib CoqlibExtra.
+Require Import Maps MapsExtra.
+Require Import Integers Floats Values AST Globalenvs.
+Require Import Errors Behaviors Smallstep.
+Require Import Language Linker.
+Require Import Tree.
+Require Import LinkerBasicproof Sig.
+Require Import SepcompRel.
+
+Require SimplExprproof.
+Require Selectionproof.
+Require Tailcallproof.
+Require Inliningproof.
+Require Renumberproof.
+Require Constpropproof.
+Require CSEproof.
+Require Deadcodeproof.
+Require Import Compiler.
+Require Import CompilerExtra.
+Require Import sflib.
+
+Set Implicit Arguments.
+
+(** Lemma on applies *)
+
+Lemma apply_partial_inversion:
+  forall A B (a:res A) (f:A -> res B) (b:B),
+    (exists a0, a = OK a0 /\ f a0 = OK b) <-> apply_partial _ _ a f = OK b.
+Proof.
+  constructor; intros.
+  - destruct H as [? [? ?]]. subst. auto.
+  - destruct a; inv H. eexists. split; eauto.
+Qed.
+
+Lemma apply_total_inversion:
+  forall A B (a:res A) (f:A -> B) (b:B),
+    (exists a0, a = OK a0 /\ f a0 = b) <-> apply_total _ _ a f = OK b.
+Proof.
+  constructor; intros.
+  - destruct H as [? [? ?]]. subst. auto.
+  - destruct a; inv H. eexists. split; eauto.
+Qed.
+
+Ltac clarify :=
+  repeat (unfold time, print in *;
+          try match goal with
+                | [TRANSF: Tree.Forall2 (fun _ _ => apply_partial _ _ _ _ = OK _) _ _ |- _] =>
+                  eapply Tree.Forall2_compat in TRANSF; [|intros; apply apply_partial_inversion; fail]
+                | [TRANSF: Tree.Forall2 (fun _ _ => apply_total _ _ _ _ = OK _) _ _ |- _] =>
+                  eapply Tree.Forall2_compat in TRANSF; [|intros; apply apply_total_inversion; fail]
+                | [TRANSF: Tree.Forall2 (fun a b => OK a = OK b) _ _ |- _] =>
+                  eapply Tree.Forall2_compat in TRANSF; [|instantiate (1 := eq); constructor; intro X; inv X; auto; fail]
+                | [TRANSF: Tree.Forall2 (fun a b => a = b) _ _ |- _] =>
+                  eapply Tree.Forall2_compat in TRANSF; [|instantiate (1 := eq); constructor; intro X; inv X; auto; fail]
+                | [TRANSF: Tree.Forall2 (fun _ _ => exists _, _ /\ _) _ _ |- _] =>
+                  let p := fresh "p" in
+                  let T := fresh "T" in
+                  apply Tree.Forall2_split in TRANSF; destruct TRANSF as [p [T TRANSF]]
+                | [TRANSF: Tree.Forall2 eq _ _ |- _] =>
+                  apply Tree.Forall2_eq in TRANSF; subst
+              end).
+
+Definition rtl_opt_tree := Tree.change_one optimize_rtl_program.
+
+Lemma rtl_opt_tree_destruct:
+  forall tr tr' (ROPTT: rtl_opt_tree tr tr'),
+    << TAILCALL: Tree.Forall2 (fun p1 p2 => (Tailcall.transf_program p1 = p2) \/ p1 = p2) tr tr' >>
+    \/  << INLINING: Tree.Forall2 (fun p1 p2 => (Inlining.transf_program p1 = OK p2) \/ p1 = p2) tr tr' >>
+    \/  << RENUMBER: Tree.Forall2 (fun p1 p2 => (Renumber.transf_program p1 = p2) \/ p1 = p2) tr tr' >>
+    \/  << CONSTPROP: Tree.Forall2 (fun p1 p2 => (Constprop.transf_program p1 = p2) \/ p1 = p2) tr tr' >>
+    \/  << CSE: Tree.Forall2 (fun p1 p2 => (CSE.transf_program p1 = OK p2) \/ p1 = p2) tr tr' >>
+    \/  << DEADCODE: Tree.Forall2 (fun p1 p2 => (Deadcode.transf_program p1 = OK p2) \/ p1 = p2) tr tr' >>.
+Proof.
+  intros. induction ROPTT.
+  - inv REL; [|right|right;right|right;right;right|right;right;right;right |right;right;right;right;right ]; [left|left|left|left|left| ]; constructor; auto.
+  - des; [|right|right;right|right;right;right|right;right;right;right |right;right;right;right;right ]; [left|left|left|left|left|];
+    (constructor; auto; eapply Tree.Forall2_implies;
+    [ intros; right; apply H | apply Tree.Tree_Forall2_eq_same]).
+  - des; [|right|right;right|right;right;right|right;right;right;right |right;right;right;right;right ]; [left|left|left|left|left|];
+    (constructor; auto; eapply Tree.Forall2_implies;
+    [ intros; right; apply H | apply Tree.Tree_Forall2_eq_same]).
+Qed.
+
+Ltac simplify :=
+  intros; subst;
+  repeat match goal with
+           | [H: OK _ = OK _ |- _] => inv H
+           | [H: bind _ _ = OK _ |- _] => monadInv H
+           | [H: _ /\ _ |- _] => destruct H
+         end;
+  subst; auto.
+
+Lemma rtl_opt_tree_reduce_simulation:
+  forall tr tr' rtlprog
+         (ROPT1T: rtl_opt_tree tr tr')
+         (REDUCE: Tree.reduce (link_program Language.Language_RTL) tr = Some rtlprog),
+  exists rtlprog'
+    (Hrtlsim': forward_simulation (RTL.semantics rtlprog) (RTL.semantics rtlprog')),
+    << Hrtlprog': Tree.reduce (link_program Language.Language_RTL) tr' = Some rtlprog' >>.
+Proof.
+  intros.
+  apply rtl_opt_tree_destruct in ROPT1T. des.
+  - eapply Tree.Forall2_implies in TAILCALL; [|apply Tailcallproof.Tailcall_sepcomp_rel].
+    eapply Tree.Forall2_reduce in TAILCALL; eauto; [|eapply (@link_program_sepcomp_rel Language.Language_RTL Language.Language_RTL id)]; simplify.
+    + destruct TAILCALL as [rtlprog1 [Hrtlprog1 Hrtlsim1]].
+      apply Tailcallproof.transf_program_correct in Hrtlsim1. eexists. eauto.
+    + des; subst; [apply Tailcall_sig | auto].
+  - eapply Tree.Forall2_implies in INLINING; [|apply Inliningproof.Inlining_sepcomp_rel].
+    eapply Tree.Forall2_reduce in INLINING; eauto; [|eapply (@link_program_sepcomp_rel Language.Language_RTL Language.Language_RTL id)]; simplify.
+    + destruct INLINING as [rtlprog1 [Hrtlprog1 Hrtlsim1]].
+      apply Inliningproof.transf_program_correct in Hrtlsim1. eexists. eauto.
+    + des; subst; [eapply Inlining_sig|]; eauto.
+  - eapply Tree.Forall2_implies in RENUMBER; [|apply Renumberproof.Renumber_sepcomp_rel].
+    eapply Tree.Forall2_reduce in RENUMBER; eauto; [|eapply (@link_program_sepcomp_rel Language.Language_RTL Language.Language_RTL id)]; simplify.
+    + destruct RENUMBER as [rtlprog1 [Hrtlprog1 Hrtlsim1]].
+      apply Renumberproof.transf_program_correct in Hrtlsim1. eexists. eauto.
+    + des; subst; auto.
+  - eapply Tree.Forall2_implies in CONSTPROP; [|apply Constpropproof.Constprop_sepcomp_rel].
+    eapply Tree.Forall2_reduce in CONSTPROP; eauto; [|eapply (@link_program_sepcomp_rel Language.Language_RTL Language.Language_RTL id)]; simplify.
+    + destruct CONSTPROP as [rtlprog1 [Hrtlprog1 Hrtlsim1]].
+      apply Constpropproof.transf_program_correct in Hrtlsim1. eexists. eauto.
+    + des; subst; auto.
+  - eapply Tree.Forall2_implies in CSE; [|apply CSEproof.CSE_sepcomp_rel].
+    eapply Tree.Forall2_reduce in CSE; eauto; [|eapply (@link_program_sepcomp_rel Language.Language_RTL Language.Language_RTL id)]; simplify.
+    + destruct CSE as [rtlprog1 [Hrtlprog1 Hrtlsim1]].
+      apply CSEproof.transf_program_correct in Hrtlsim1. eexists. eauto.
+    + des; subst; [eapply CSE_sig|]; eauto.
+  - eapply Tree.Forall2_implies in DEADCODE; [|apply Deadcodeproof.Deadcode_sepcomp_rel].
+    eapply Tree.Forall2_reduce in DEADCODE; eauto; [|eapply (@link_program_sepcomp_rel Language.Language_RTL Language.Language_RTL id)]; simplify.
+    + destruct DEADCODE as [rtlprog1 [Hrtlprog1 Hrtlsim1]].
+      apply Deadcodeproof.transf_program_correct in Hrtlsim1. eexists. eauto.
+    + des; subst; [eapply Deadcode_sig|]; eauto.
+Qed.
+
+Inductive match_state_refl (s:semantics): forall (st1 st2:state s), Prop :=
+| match_state_refl_intro: forall st, match_state_refl s st st.
+
+Lemma forward_simulation_refl:
+  forall sem, forward_simulation sem sem.
+Proof.
+  intros.
+  eapply forward_simulation_step; eauto; intros.
+  - eexists. split; eauto. apply (match_state_refl_intro _ s1).
+  - inv H; auto.
+  - eexists. inv H0. split; eauto. constructor.
+Qed.
+
+Lemma optimize_rtl_program_reduce_simulation:
+  forall (rtlprog: RTL.program)
+         (tr1 tr2: Tree.t RTL.program)
+         (REDUCE: Tree.reduce (link_program Language.Language_RTL) tr1 = Some rtlprog)
+         (ROPT: rtc rtl_opt_tree tr1 tr2),
+  exists rtlprog'
+         (Hrtlsim': forward_simulation (RTL.semantics rtlprog) (RTL.semantics rtlprog')),
+    << Hrtlprog': Tree.reduce (link_program Language.Language_RTL) tr2 = Some rtlprog' >>.
+Proof.
+  intros. generalize dependent rtlprog.
+  induction ROPT; intros.
+  - exploit rtl_opt_tree_reduce_simulation; eauto.
+  - exists rtlprog. exists (forward_simulation_refl (RTL.semantics rtlprog)); eauto.
+  - exploit IHROPT1; eauto. intros. des.
+    exploit IHROPT2; eauto. intros. des.
+    exists rtlprog'0.
+    exists (compose_forward_simulation Hrtlsim' Hrtlsim'0); eauto.
+Qed.
+
+Lemma linker_correct_determinate_forward
+        ctree asmtree cprog
+        (CLINK: Tree.reduce (link_program Language.Language_C) ctree = Some cprog)
+        (TRANSF: Tree.Forall2 compile_c_program ctree asmtree):
+  exists (asmprog:Asm.program)
+    (_:forward_simulation (Cstrategy.semantics cprog) (Asm.semantics asmprog)),
+    Tree.reduce (link_program Language.Language_Asm) asmtree = Some asmprog.
+Proof.
+  repeat intro.
+
+  (* C *)
+  unfold compile_c_program in TRANSF.
+  eapply Tree.Tree_Forall2_split2 in TRANSF. des.
+
+  unfold transf_c_program_to_rtl in TRANSF. clarify.
+  eapply Tree.Forall2_implies in T; [|apply SimplExprproof.SimplExpr_sepcomp_rel].
+  eapply Tree.Forall2_reduce in T; eauto;
+    [|eapply (@link_program_sepcomp_rel Language.Language_C Language.Language_Clight id)]; simplify;
+    [|apply SimplExpr_sig; auto].
+  destruct T as [clightprog [Hclightprog Hclightsim]].
+  apply SimplExprproof.transl_program_correct in Hclightsim.
+
+  (* Clight *)
+  unfold transf_clight_program_to_rtl in TRANSF. clarify.
+
+  eapply Tree.Forall2_reduce in T1; eauto;
+    [|eapply (transform_partial_program2_link_program Language.Language_Clight Language.Language_Clight)];
+    [|apply SimplLocals_sig].
+  destruct T1 as [clight2prog [Hclight2prog Hclight2sim]].
+  apply SimplLocalsproof.transf_program_correct in Hclight2sim.
+
+  eapply Tree.Forall2_reduce in T0; eauto;
+    [|eapply (transform_partial_program2_link_program Language.Language_Clight Language.Language_Csharpminor)];
+    [|apply Cshmgen_sig].
+  destruct T0 as [csharpminorprog [Hsharpminorprog Hsharpminorsim]].
+  apply Cshmgenproof.transl_program_correct in Hsharpminorsim.
+
+  eapply Tree.Forall2_reduce in T; eauto;
+    [|eapply (transform_partial_program2_link_program Language.Language_Csharpminor Language.Language_Cminor)];
+    [|apply globfun_linkable_transf_partial_fundef];
+    [|apply Cminorgen_sig].
+  destruct T as [cminorprog [Hcminorprog Hcminorsim]].
+  apply Cminorgenproof.transl_program_correct in Hcminorsim.
+
+  (* Cminor *)
+  unfold transf_cminor_program_to_rtl in TRANSF. clarify.
+
+  assert (Hcheck_helpers: SelectLong.check_helpers (Genv.globalenv cminorprog) = OK tt).
+  {
+    exploit Tree.Forall_reduce; [| |eauto|].
+    - eapply Selectionproof.link_program_check_helpers.
+    - clear -T. revert p5 T.
+      induction p; intros; inv T; econstructor; eauto.
+      monadInv Hpred. destruct x. auto.
+    - auto.
+  }
+
+  eapply Tree.Forall2_implies in T; [|apply Selectionproof.Selection_sepcomp_rel].
+  eapply Tree.Forall2_reduce in T; eauto;
+    [|eapply (@link_program_sepcomp_rel Language.Language_Cminor Language.Language_CminorSel id)]; simplify;
+    [|eapply Selection_sig; eauto].
+
+  destruct T as [cminorselprog [Hcminorselprog Hcminorselsim]].
+  apply Selectionproof.transl_program_correct in Hcminorselsim;
+    eauto using Selectionproof.check_helpers_correct.
+
+  eapply Tree.Forall2_reduce in TRANSF; eauto;
+    [|eapply (transform_partial_program2_link_program Language.Language_CminorSel Language.Language_RTL)];
+    [|apply globfun_linkable_transf_partial_fundef];
+    [|apply RTLgen_sig].
+  destruct TRANSF as [rtlprog0 [Hrtlprog0 Hrtlsim0]].
+  apply RTLgenproof.transf_program_correct in Hrtlsim0.
+
+(* RTL *)
+  exploit optimize_rtl_program_reduce_simulation.
+  eauto. apply Tree.Tree_Forall2_rtc_rel_rtc_change_one. eauto.
+  intros. des.
+  unfold transf_rtl_program_to_asm in TRANSF1. clarify.
+
+  eapply Tree.Forall2_reduce in T5; eauto;
+    [|eapply (transform_partial_program2_link_program Language.Language_RTL Language.Language_LTL)];
+    [|apply globfun_linkable_transf_partial_fundef];
+    [|apply Allocation_sig].
+  destruct T5 as [ltlprog0 [Hltlprog0 Hltlsim0]].
+  apply Allocproof.transf_program_correct in Hltlsim0.
+
+  eapply Tree.Forall2_reduce in T3; eauto;
+    [|eapply (transform_program_link_program); auto].
+  destruct T3 as [ltlprog1 [Hltlprog1 Hltlsim1]]. subst.
+  generalize (Tunnelingproof.transf_program_correct ltlprog0) as Hltlsim1. intro.
+
+  eapply Tree.Forall2_reduce in T2; eauto;
+    [|eapply (transform_partial_program2_link_program Language.Language_LTL Language.Language_Linear)];
+    [|apply globfun_linkable_transf_partial_fundef];
+    [|apply Linearize_sig].
+  destruct T2 as [linearprog0 [Hlinearprog0 Hlinearsim0]].
+  apply Linearizeproof.transf_program_correct in Hlinearsim0.
+
+  eapply Tree.Forall2_reduce in T1; eauto;
+    [|eapply (transform_program_link_program); auto].
+  destruct T1 as [linearprog1 [Hlinearprog1 Hlinearsim1]]. subst.
+  generalize (CleanupLabelsproof.transf_program_correct linearprog0) as Hlinearsim1. intro.
+
+  eapply Tree.Forall2_reduce in T0; eauto;
+    [|eapply (transform_partial_program2_link_program Language.Language_Linear Language.Language_Mach)];
+    [|apply globfun_linkable_transf_partial_fundef];
+    [|apply Stacking_sig].
+  destruct T0 as [machprog [Hmachprog Hmachsim]].
+  eapply Stackingproof.transf_program_correct in Hmachsim; eauto;
+    [|eexact Asmgenproof.return_address_exists; eassumption].
+
+  eapply Tree.Forall2_reduce in TRANSF1; eauto;
+    [|eapply (transform_partial_program2_link_program Language.Language_Mach Language.Language_Asm)];
+    [|apply globfun_linkable_transf_partial_fundef];
+    [|apply Asmgen_sig].
+  destruct TRANSF1 as [asmprog [Hasmprog Hasmsim]].
+  eapply Asmgenproof.transf_program_correct in Hasmsim; eauto.
+
+  (* epilogue *)
+  exists asmprog. eexists; auto.
+  repeat (auto; try (eapply compose_forward_simulation; [|eauto; fail])).
+Qed.
+
+Lemma linker_correct_determinate
+        ctree asmtree cprog
+        (CLINK: Tree.reduce (link_program Language.Language_C) ctree = Some cprog)
+        (TRANSF: Tree.Forall2 compile_c_program ctree asmtree):
+  exists (asmprog:Asm.program)
+    (_:backward_simulation (atomic (Cstrategy.semantics cprog)) (Asm.semantics asmprog)),
+    Tree.reduce (link_program Language.Language_Asm) asmtree = Some asmprog.
+Proof.
+  exploit linker_correct_determinate_forward; eauto.
+  intros [asmprog [Hsim Hasmprog]]. exists asmprog.
+  eexists; auto.
+  apply forward_to_backward_simulation.
+  apply factor_forward_simulation. auto. eapply sd_traces. eapply Asm.semantics_determinate.
+  apply atomic_receptive. apply Cstrategy.semantics_strongly_receptive.
+  apply Asm.semantics_determinate.
+Qed.
+
+Theorem linker_correct
+        ctree asmtree cprog
+        (CLINK: Tree.reduce (link_program Language.Language_C) ctree = Some cprog)
+        (TRANSF: Tree.Forall2 compile_c_program ctree asmtree):
+  exists (asmprog:Asm.program)
+    (_:backward_simulation (Csem.semantics cprog) (Asm.semantics asmprog)),
+    Tree.reduce (link_program Language.Language_Asm) asmtree = Some asmprog.
+Proof.
+  exploit linker_correct_determinate; eauto.
+  intros [asmprog [Hsim Hasmprog]]. exists asmprog.
+  eexists; eauto.
+  apply compose_backward_simulation with (atomic (Cstrategy.semantics cprog)).
+  eapply sd_traces; eapply Asm.semantics_determinate.
+  apply factor_backward_simulation. 
+  apply Cstrategy.strategy_simulation.
+  apply Csem.semantics_single_events.
+  eapply ssr_well_behaved; eapply Cstrategy.semantics_strongly_receptive.
+  exact Hsim.
+Qed.
