sepcomp/status.sh
@@ -1,4 +1,0 @@
-#!/usr/bin/env bash
-
-egrep -r "(dmit|TODO|todo)" .
-
